move PlusFold into Contract

theories/Contract.v
@@ -305,7 +305,7 @@ Qed.
 
 
 
-(*Some dependencies used by ParallelContract and PlusFold*)
+(***********************Some dependencies used by ParallelContract and ContractEquation******************)
 
 Lemma plus_comm : forall (c1 c2 : Contract),(forall s, s ==~ (c1 _+_ c2) <-> s ==~ (c2 _+_ c1)).
 Proof.
@@ -357,6 +357,66 @@ split.
 - intros. repeat rewrite comp_iff_oper in *.
 apply plus_or_oper in H. apply H.
 - intros. destruct H. { now apply MPlusL. } { now apply MPlusR. }
+Qed.
+
+
+Fixpoint plus_fold (l : list Contract) : Contract :=
+match l with
+| [] => Failure
+| c ::l => c _+_ (plus_fold l)
+end.
+
+
+Lemma plus_fold_app : forall (s:Trace)(l1 l2 : list Contract), 
+s ==~ plus_fold (l1 ++ l2) <-> s ==~ (plus_fold l1) _+_ (plus_fold l2).
+Proof.
+intro. induction l1.
+- intros. split.
+  * intros. simpl in H. auto.
+  * intros. simpl. simpl in H. inversion H. {  inversion H2. } assumption.
+- intros. split.
+  * intros. simpl in *. apply plus_or in H as [H | H] ; auto.
+    specialize IHl1 with l2. apply IHl1 in H. apply plus_assoc. auto.
+  * intros. simpl in *. apply plus_assoc in H. apply plus_or in H as [H | H].
+    ** auto.
+    ** apply MPlusR. apply IHl1. assumption.
+Qed.
+
+
+Lemma in_plus_fold : forall (s : Trace)(l : list Contract), s ==~ plus_fold l <-> 
+(exists c, In c l /\ s ==~ c).
+Proof.
+intros. split.
+- induction l.
+  * intros. simpl in H. inversion H.
+  * intros. simpl in H. apply plus_or in H as [H | H].
+    ** exists a. split. apply in_eq. assumption.
+    ** apply IHl in H as [c' [P1 P2]]. exists c'. split ; auto using  in_cons.
+- intros. destruct H as [ c' [P1 P2]]. induction l.
+  * destruct P1.
+  * apply in_inv in P1 as [P1 | P1].
+    ** simpl. rewrite P1. auto.
+    ** simpl. auto.
+Qed.
+
+
+
+
+
+
+Fixpoint seq_fold (l : list Contract) :=
+match l with
+| [] => Success
+| a::l' => a _;_ (seq_fold l')
+end.
+
+
+
+Lemma seq_fold_map : forall (s:Trace), s ==~ seq_fold (map Event s).
+Proof.
+induction s.
+- simpl. auto.
+- simpl. assert (HA: a::s = [a]++s). { reflexivity. } rewrite HA. constructor; auto.
 Qed.
 
 
