theories/NormalizedParallelContract.v
@@ -1,6 +1,5 @@
 Require Import CSL.Contract.
 Require Import CSL.Order.
-Require Import CSL.PlusFold.
 Require Import Lists.List.
 Require Import Sorting.Permutation.
 Require Import Sorting.Mergesort.
@@ -9,3 +8,5 @@ Require Import Bool.Bool.
 Require Import Bool.Sumbool.
 Require Import List Setoid Permutation Sorted Orders.
 Import ListNotations.
+
+
